src/xor/tseitin_xor.lean
@@ -30,14 +30,15 @@ open gensym
 
 open nat
 open list
+open list.perm
 open assignment
 open function
 
 namespace tseitin_xor
 
-variables {l : list (literal V)} {g : gensym V} {k : nat} {v : V} {τ : assignment V}
+variables {l : list (literal V)} {g : gensym V} {k : nat} (hk : k ≥ 3) {v : V} {τ : assignment V}
 
-lemma disjoint_fresh_of_disjoint (hk : k ≥ 3) : disjoint g.stock (clause.vars l) → 
+lemma disjoint_fresh_of_disjoint : disjoint g.stock (clause.vars l) → 
   disjoint g.fresh.2.stock (clause.vars ((Pos g.fresh.1) :: (l.drop (k - 1)))) :=
 begin
   intro h,
@@ -61,36 +62,37 @@ begin
   rcases exists_append_of_gt_length hl with ⟨x₁, x₂, rfl, hl₁⟩,
   simp only [hl₁, length_drop, length_append],
   rw [add_comm k x₂.length, nat.add_sub_assoc (nat.sub_le k 1),
-      nat.sub_sub_self (nat.le_of_add_le_right hk), add_assoc],
+      nat.sub_sub_self (le_of_add_le_right hk), add_assoc],
   apply add_lt_add_left,
   exact succ_le_iff.mp hk,
 end
 
--- Note: l and g can be made implicit args
-def linear_xor (hk : k ≥ 3) : list (literal V) → gensym V → cnf V
-| l g := if h : length l ≤ k then direct_xor l else
-           have length ((Pos g.fresh.1) :: (l.drop (k - 1))) < length l,
-             from (drop_len_lt _ hk (not_le.mp h)),
-           (direct_xor (l.take (k - 1) ++ [(Neg g.fresh.1)])) ++
-           (linear_xor ((Pos g.fresh.1) :: (l.drop (k - 1))) (g.fresh.2))
+variables {p : list (literal V) → list (literal V)} (hp : ∀ l, perm l (p l))
+
+def tseitin_xor : list (literal V) → gensym V → cnf V
+| l g :=  if h : length l ≤ k then direct_xor l else
+          have length (p (Pos g.fresh.1 :: (l.drop (k - 1)))) < length l,
+            from (perm.length_eq (hp (Pos g.fresh.1 :: (l.drop (k - 1))))) ▸ 
+              (drop_len_lt _ hk (not_le.mp h)),
+          (direct_xor (l.take (k - 1) ++ [(Neg g.fresh.1)])) ++
+          (tseitin_xor (p (Pos g.fresh.1 :: (l.drop (k - 1)))) g.fresh.2)
 using_well_founded {
   rel_tac := λ a b, `[exact ⟨_, measure_wf (λ σ, list.length σ.1)⟩],
   dec_tac := tactic.assumption
 }
 
-lemma linear_base_case (hk : k ≥ 3) :
-  length l ≤ k → linear_xor hk l g = direct_xor l :=
-assume h, by { rw linear_xor, simp only [h, if_true] }
+lemma tseitin_base_case : length l ≤ k → tseitin_xor hk hp l g = direct_xor l :=
+assume h, by { rw tseitin_xor, simp only [h, if_true] }
 
-theorem mem_linear_xor_vars_of_mem_vars (hk : k ≥ 3)
+theorem mem_tseitin_xor_vars_of_mem_vars
   (hdis : disjoint g.stock (clause.vars l)) :
-  v ∈ (clause.vars l) → v ∈ (linear_xor hk l g).vars :=
+  v ∈ (clause.vars l) → v ∈ (tseitin_xor hk hp l g).vars :=
 begin
   induction l using strong_induction_on_lists with l ih generalizing g,
   by_cases hl : length l ≤ k,
-  { rw linear_base_case hk hl, rw vars_direct_xor, exact id },
+  { rw [tseitin_base_case hk hp hl, vars_direct_xor], exact id },
   { intro h,
-    rw linear_xor,
+    rw tseitin_xor,
     simp [hl],
     rw [← take_append_drop (k - 1) l, clause.vars_append] at h,
     rw cnf.vars_append,
@@ -100,20 +102,23 @@ begin
       exact finset.mem_union_left _ h },
     { rw not_le at hl,
       have h₁ := drop_len_lt (Pos g.fresh.1) hk hl,
-      have h₂ := disjoint_fresh_of_disjoint hk hdis,
-      have := ih _ h₁ h₂ (mem_vars_cons_of_mem_vars _ h),
-      exact finset.mem_union_right _ this } }
+      have h₂ := disjoint_fresh_of_disjoint hdis,
+      rw perm.length_eq (hp (Pos g.fresh.1 :: drop (k - 1) l)) at h₁,
+      rw vars_perm (hp (Pos g.fresh.1 :: drop (k - 1) l)) at h₂,
+      have := ih _ h₁ h₂,
+      rw ← clause.vars_perm (hp (Pos g.fresh.1 :: drop (k - 1) l)) at this,
+      exact finset.mem_union_right _ (this (mem_vars_cons_of_mem_vars _ h)) } }
 end
 
-theorem not_mem_linear_xor_vars_of_not_mem_vars_of_not_mem_stock 
-  (hk : k ≥ 3) (hdis : disjoint g.stock (clause.vars l)) :
-  v ∉ (clause.vars l) → v ∉ g.stock → v ∉ (linear_xor hk l g).vars :=
+theorem not_mem_tseitin_xor_vars_of_not_mem_vars_of_not_mem_stock
+  (hdis : disjoint g.stock (clause.vars l)) :
+  v ∉ (clause.vars l) → v ∉ g.stock → v ∉ (tseitin_xor hk hp l g).vars :=
 begin
   induction l using strong_induction_on_lists with l ih generalizing g,
   by_cases hl : length l ≤ k,
-  { rw [linear_base_case hk hl, vars_direct_xor l], tautology },
+  { rw [tseitin_base_case hk hp hl, vars_direct_xor l], tautology },
   { intros hvars hg,
-    rw linear_xor,
+    rw tseitin_xor,
     simp [hl],
     rw cnf.vars_append,
     apply finset.not_mem_union.mpr,
@@ -129,7 +134,7 @@ begin
         rw hcon at hg,
         exact absurd (fresh_mem_stock g) hg } },
     { have h₁ := drop_len_lt (Pos g.fresh.1) hk (not_le.mp hl),
-      have h₂ := disjoint_fresh_of_disjoint hk hdis,
+      have h₂ := disjoint_fresh_of_disjoint hdis,
       have h₃ : v ∉ clause.vars (Pos g.fresh.1 :: drop (k - 1) l),
       { simp [clause.vars, var],
         rintros (rfl | h),
@@ -138,27 +143,32 @@ begin
       have h₄ : v ∉ g.fresh.2.stock,
       { intro hcon,
         exact hg ((fresh_stock_subset g) hcon) },
+      rw perm.length_eq (hp (Pos g.fresh.1 :: drop (k - 1) l)) at h₁,
+      rw vars_perm (hp (Pos g.fresh.1 :: drop (k - 1) l)) at h₂ h₃,
       exact ih _ h₁ h₂ h₃ h₄ } }
 end
 
-lemma linear_forward (hk : k ≥ 3) (hdis : disjoint g.stock (clause.vars l)) :
-  Xor.eval τ l = tt → ∃ (σ : assignment V), 
-  (linear_xor hk l g).eval σ = tt ∧ (τ≡(clause.vars l)≡σ) :=
+lemma tseitin_forward (hdis : disjoint g.stock (clause.vars l)) : 
+  Xor.eval τ l = tt → ∃ (σ : assignment V),
+  (tseitin_xor hk hp l g).eval σ = tt ∧ (eqod τ σ (clause.vars l)) :=
 begin
   intro he,
   induction l using strong_induction_on_lists with l ih generalizing g τ,
   by_cases hl : length l ≤ k,
-  { use τ, rw [linear_base_case hk hl, eval_direct_xor_eq_eval_Xor], simp [he] },
-  { rw [eval_eq_bodd_count_tt,
+  { use τ, rw [tseitin_base_case hk hp hl, eval_direct_xor_eq_eval_Xor], simp [he] },
+  {
+    rw [eval_eq_bodd_count_tt,
       ← (take_append_drop (k - 1) l), count_tt_append, bodd_add] at he,
 
     have hnotmem := set.disjoint_left.mp hdis (g.fresh_mem_stock),
     have h₁ := drop_len_lt (Pos g.fresh.1) hk (not_le.mp hl),
-    have h₂ := disjoint_fresh_of_disjoint hk hdis,
+    have h₂ := disjoint_fresh_of_disjoint hdis,
+    rw perm.length_eq (hp (Pos g.fresh.1 :: drop (k - 1) l)) at h₁,
+    rw vars_perm (hp (Pos g.fresh.1 :: drop (k - 1) l)) at h₂,
     have htakevars := vars_subset_of_subset (take_subset (k - 1) l),
     have hdropvars := vars_subset_of_subset (drop_subset (k - 1) l),
 
-    rw linear_xor,
+    rw tseitin_xor,
     simp [hl, cnf.eval_append],
 
     -- Case on the truth value of the last n - k + 1 variables
@@ -169,16 +179,17 @@ begin
       have : bodd (clause.count_tt γ (Pos g.fresh.1 :: drop (k - 1) l)) = tt,
       { simp only [count_tt_cons, literal.eval, hg, cond,
           ← count_tt_eq_of_eqod (eqod_subset hdropvars heqod), he] },
-      rw [← eval_eq_bodd_count_tt] at this,
+      rw [← eval_eq_bodd_count_tt, eval_eq_of_perm (hp (Pos g.fresh.1 :: drop (k - 1) l))] at this,
 
       -- Apply the induction hypothesis
       rcases (ih _ h₁ h₂ this) with ⟨γ₂, he₂, hg₂⟩,
 
-      have heqod₂ : eqod (assignment.ite (cnf.vars (linear_xor hk (Pos g.fresh.1 :: (l.drop (k - 1))) g.fresh.2)) γ₂ γ) γ (clause.vars l),
+      have heqod₂ : eqod (assignment.ite (cnf.vars (tseitin_xor hk hp (p (Pos g.fresh.1 :: (l.drop (k - 1)))) g.fresh.2)) γ₂ γ) γ (clause.vars l),
       { intros v hv,
         by_cases hmem : v ∈ clause.vars (l.drop (k - 1)),
         { have h₃ := mem_vars_cons_of_mem_vars (Pos g.fresh.1) hmem,
-          rw [ite_pos (mem_linear_xor_vars_of_mem_vars hk h₂ h₃), hg₂ v h₃] },
+          rw vars_perm (hp (Pos g.fresh.1 :: drop (k - 1) l)) at h₃,
+          rw [ite_pos (mem_tseitin_xor_vars_of_mem_vars hk hp h₂ h₃), hg₂ v h₃] },
         { have hdis₂ := set.disjoint_right.mp hdis hv,
           have hne : v ≠ g.fresh.1,
           { intro hcon,
@@ -188,41 +199,43 @@ begin
             rintros (hcon | hcon),
             { exact hne hcon },
             { exact hmem hcon } },
+          rw vars_perm (hp (Pos g.fresh.1 :: drop (k - 1) l)) at this,
           have hstock : v ∉ g.fresh.2.stock,
           { intro hcon,
             exact hdis₂ ((fresh_stock_subset g) hcon) },
-          rw ite_neg (not_mem_linear_xor_vars_of_not_mem_vars_of_not_mem_stock hk h₂ this hstock) } },
+          rw ite_neg (not_mem_tseitin_xor_vars_of_not_mem_vars_of_not_mem_stock hk hp h₂ this hstock) } },
         
-      use assignment.ite (cnf.vars (linear_xor hk (Pos g.fresh.1 :: (l.drop (k - 1))) g.fresh.2)) γ₂ γ,
+      use assignment.ite (cnf.vars (tseitin_xor hk hp (p (Pos g.fresh.1 :: (l.drop (k - 1)))) g.fresh.2)) γ₂ γ,
       split,
       { split,
         { simp [eval_direct_xor_eq_eval_Xor, eval_eq_bodd_count_tt, 
             count_tt_append, bodd_add, literal.eval, hg],
           have : g.fresh.1 ∈ clause.vars (Pos g.fresh.1 :: (l.drop (k - 1))),
           { exact mem_vars_cons_self _ _ },
-          simp [ite_pos (mem_linear_xor_vars_of_mem_vars hk h₂ this), 
+          rw vars_perm (hp (Pos g.fresh.1 :: drop (k - 1) l)) at this,
+          simp [ite_pos (mem_tseitin_xor_vars_of_mem_vars hk hp h₂ this), 
             ← (hg₂ g.fresh.1 this), hg,
             count_tt_eq_of_eqod (eqod_subset htakevars heqod₂),
             ← count_tt_eq_of_eqod (eqod_subset htakevars heqod), hc] },
         { exact he₂ ▸ eval_eq_cnf_of_eqod (ite_eqod _ _ _) } },
       { exact eqod.trans heqod (heqod₂.symm) } },
-    {
-      simp only [hc, bnot_eq_true_eq_eq_ff, tt_bxor] at he,
+    { simp only [hc, bnot_eq_true_eq_eq_ff, tt_bxor] at he,
         rcases exists_eqod_and_eq_of_not_mem τ tt hnotmem with ⟨γ, heqod, hg⟩,
         have : bodd (clause.count_tt γ (Pos g.fresh.1 :: drop (k - 1) l)) = tt,
         { simp only [count_tt_cons, literal.eval, hg, cond, 
             ← count_tt_eq_of_eqod (eqod_subset hdropvars heqod), he, bodd_succ, 
             bodd_add, bodd_zero, bool.bnot_false, bool.bxor_ff_right], },
-        rw [← eval_eq_bodd_count_tt] at this,
+        rw [← eval_eq_bodd_count_tt, eval_eq_of_perm (hp (Pos g.fresh.1 :: drop (k - 1) l))] at this,
 
         -- Apply the induction hypothesis
         rcases (ih _ h₁ h₂ this) with ⟨γ₂, he₂, hg₂⟩,
 
-        have heqod₂ : eqod (assignment.ite (cnf.vars (linear_xor hk (Pos g.fresh.1 :: (l.drop (k - 1))) g.fresh.2)) γ₂ γ) γ (clause.vars l),
+        have heqod₂ : eqod (assignment.ite (cnf.vars (tseitin_xor hk hp (p (Pos g.fresh.1 :: (l.drop (k - 1)))) g.fresh.2)) γ₂ γ) γ (clause.vars l),
         { intros v hv,
           by_cases hmem : v ∈ clause.vars (l.drop (k - 1)),
           { have h₃ := mem_vars_cons_of_mem_vars (Pos g.fresh.1) hmem,
-            rw [ite_pos (mem_linear_xor_vars_of_mem_vars hk h₂ h₃), hg₂ v h₃] },
+            rw vars_perm (hp (Pos g.fresh.1 :: drop (k - 1) l)) at h₃,
+            rw [ite_pos (mem_tseitin_xor_vars_of_mem_vars hk hp h₂ h₃), hg₂ v h₃] },
           { have hdis₂ := set.disjoint_right.mp hdis hv,
             have hne : v ≠ g.fresh.1,
             { intro hcon,
@@ -232,19 +245,21 @@ begin
               rintros (hcon | hcon),
               { exact hne hcon },
               { exact hmem hcon } },
+            rw vars_perm (hp (Pos g.fresh.1 :: drop (k - 1) l)) at this,
             have hstock : v ∉ g.fresh.2.stock,
             { intro hcon,
               exact hdis₂ ((fresh_stock_subset g) hcon) },
-            rw ite_neg (not_mem_linear_xor_vars_of_not_mem_vars_of_not_mem_stock hk h₂ this hstock) } },
+            rw ite_neg (not_mem_tseitin_xor_vars_of_not_mem_vars_of_not_mem_stock hk hp h₂ this hstock) } },
         
-        use assignment.ite (cnf.vars (linear_xor hk (Pos g.fresh.1 :: (l.drop (k - 1))) g.fresh.2)) γ₂ γ,
+        use assignment.ite (cnf.vars (tseitin_xor hk hp (p (Pos g.fresh.1 :: (l.drop (k - 1)))) g.fresh.2)) γ₂ γ,
         split,
         { split,
           { simp [eval_direct_xor_eq_eval_Xor, eval_eq_bodd_count_tt, 
               count_tt_append, bodd_add, literal.eval, hg],
             have : g.fresh.1 ∈ clause.vars (Pos g.fresh.1 :: (l.drop (k - 1))),
             { exact mem_vars_cons_self _ _ },
-            simp [ite_pos (mem_linear_xor_vars_of_mem_vars hk h₂ this), 
+            rw vars_perm (hp (Pos g.fresh.1 :: drop (k - 1) l)) at this,
+            simp [ite_pos (mem_tseitin_xor_vars_of_mem_vars hk hp h₂ this), 
               ← (hg₂ g.fresh.1 this), hg,
               count_tt_eq_of_eqod (eqod_subset htakevars heqod₂),
               ← count_tt_eq_of_eqod (eqod_subset htakevars heqod), hc] },
@@ -252,21 +267,24 @@ begin
         { exact eqod.trans heqod heqod₂.symm } } } 
 end
 
-lemma linear_reverse (hk : k ≥ 3) (hdis : disjoint g.stock (clause.vars l)) :
-  cnf.eval τ (linear_xor hk l g) = tt → Xor.eval τ l = tt :=
+lemma tseitin_reverse (hdis : disjoint g.stock (clause.vars l)) :
+  cnf.eval τ (tseitin_xor hk hp l g) = tt → Xor.eval τ l = tt :=
 begin
   intro he,
   induction l using strong_induction_on_lists with l ih generalizing g,
   by_cases hl : length l ≤ k,
-  { rw [linear_base_case hk hl, eval_direct_xor_eq_eval_Xor] at he, exact he },
-  { rw linear_xor at he,
+  { rw [tseitin_base_case hk hp hl, eval_direct_xor_eq_eval_Xor] at he, exact he },
+  { rw tseitin_xor at he,
     simp [hl, cnf.eval_append] at he,
     rcases he with ⟨hdir, hrec⟩,
     have h₁ := drop_len_lt (Pos g.fresh.1) hk (not_le.mp hl),
-    have h₂ := disjoint_fresh_of_disjoint hk hdis,
+    have h₂ := disjoint_fresh_of_disjoint hdis,
+    rw perm.length_eq (hp (Pos g.fresh.1 :: drop (k - 1) l)) at h₁,
+    rw vars_perm (hp (Pos g.fresh.1 :: drop (k - 1) l)) at h₂,
     have ihred := ih _ h₁ h₂ hrec,
     rw eval_direct_xor_eq_eval_Xor at hdir,
     rw eval_eq_bodd_count_tt at ihred hdir |-,
+    rw ← count_tt_perm (hp (Pos g.fresh.1 :: drop (k - 1) l)) at ihred,
     have := congr_arg ((clause.count_tt τ)) (take_append_drop (k - 1) l).symm,
     have := congr_arg bodd this,
     cases hnew : (τ g.fresh.1),
@@ -278,273 +296,50 @@ begin
       exact this } }
 end
 
-theorem linear_xor_encodes_Xor (hk : k ≥ 3) (hdis : disjoint g.stock (clause.vars l)) :
-  encodes Xor (linear_xor hk l g) l :=
+theorem tseitin_xor_encodes_Xor (hdis : disjoint g.stock (clause.vars l)) :
+  encodes Xor (tseitin_xor hk hp l g) l :=
 begin
   intro τ,
   split,
-  { exact linear_forward hk hdis },
+  { exact tseitin_forward hk hp hdis },
   { rintros ⟨σ, he, heqod⟩,
     rw [← Xor.eval, eval_eq_Xor_of_eqod heqod],
-    exact linear_reverse hk hdis he }
+    exact tseitin_reverse hk hp hdis he }
 end
 
--- Note: The proofs here are symmetric with the linear encoding ones
--- If an improvement is made to the above proofs, simplify here
+def linear_perm (l : list (literal V)) : list (literal V) := l
 
-lemma drop_len_lt' (lit : literal V) (hk : k ≥ 3) :
-  length l > k → length (l.drop (k - 1) ++ [lit]) < length l :=
+lemma linear_perm_is_perm : ∀ (l : list (literal V)), l ~ linear_perm l :=
 begin
-  have : (drop (k - 1) l ++ [lit]).length = (lit :: drop (k - 1) l).length,
-  { simp only [length, length_append] },
-  rw this,
-  exact drop_len_lt lit hk
+  intro l,
+  rw linear_perm
 end
 
-lemma disjoint_fresh_of_disjoint' (hk : k ≥ 3) :
-  disjoint g.stock (clause.vars l) → 
-  disjoint g.fresh.2.stock (clause.vars (l.drop (k - 1) ++ [Pos g.fresh.1])) :=
+def linear_xor (l : list (literal V)) (g : gensym V) : cnf V :=
+  tseitin_xor hk linear_perm_is_perm l g
+
+theorem linear_xor_encodes_Xor (hdis : disjoint g.stock (clause.vars l)) :
+  encodes Xor (linear_xor hk l g) l :=
+tseitin_xor_encodes_Xor hk linear_perm_is_perm hdis
+
+def pooled_perm : list (literal V) → list (literal V)
+| []        := []
+| (x :: xs) := xs ++ [x]
+
+lemma pooled_perm_is_perm : ∀ (l : list (literal V)), l ~ pooled_perm l :=
 begin
-  intro h,
-  apply set.disjoint_right.mpr,
-  intros v hv,
-  simp [clause.vars, clause.vars_append] at hv,
-  rcases hv with rfl | hv,
-  { rw var,
-    exact fresh_not_mem_fresh_stock g },
-  { intro hcon,
-    rw set.disjoint_right at h,
-    have := vars_subset_of_subset (drop_subset (k - 1) l),
-    exact absurd ((fresh_stock_subset g) hcon) (h (this hv)) }
+  intro l,
+  cases l,
+  { refl },
+  { rw [pooled_perm, ← singleton_append],
+    exact perm_append_comm }
 end
 
--- Note: x and g can be made implicit args
-def pooled_xor (hk : k ≥ 3) : Π (l : list (literal V)), Π (g : gensym V),
-  (disjoint g.stock (clause.vars l)) → cnf V
-| l g hdis := if h : length l ≤ k then direct_xor l else
-                have length (l.drop (k - 1) ++ [Pos g.fresh.1]) < length l,
-                  from (drop_len_lt' _ hk (not_le.mp h)),
-                (direct_xor (l.take (k - 1) ++ [(Neg g.fresh.1)])) ++
-                (pooled_xor (l.drop (k - 1) ++ [Pos g.fresh.1]) (g.fresh.2)
-                (disjoint_fresh_of_disjoint' hk hdis))
-using_well_founded {
-  rel_tac := λ a b, `[exact ⟨_, measure_wf (λ σ, list.length σ.1)⟩],
-  dec_tac := tactic.assumption
-}
+def pooled_xor (l : list (literal V)) (g : gensym V) : cnf V :=
+  tseitin_xor hk pooled_perm_is_perm l g
 
-lemma pooled_base_case (hk : k ≥ 3) (hdis : disjoint g.stock (clause.vars l)) : 
-  length l ≤ k → pooled_xor hk l g hdis = direct_xor l :=
-assume h, by { rw pooled_xor, simp only [h, if_true] }
-
-theorem mem_pooled_xor_vars_of_mem_vars (hk : k ≥ 3)
-  (hdis : disjoint g.stock (clause.vars l)) :
-  v ∈ (clause.vars l) → v ∈ (pooled_xor hk l g hdis).vars :=
-begin
-  induction l using strong_induction_on_lists with l ih generalizing g,
-  by_cases hl : length l ≤ k,
-  { rw pooled_base_case hk hdis hl, rw vars_direct_xor, exact id },
-  { intro h,
-    rw pooled_xor,
-    simp [hl],
-    rw [← take_append_drop (k - 1) l, clause.vars_append] at h,
-    rw cnf.vars_append,
-    rcases finset.mem_union.mp h with (h | h),
-    { apply finset.mem_union_left,
-      rw [vars_direct_xor, clause.vars_append],
-      exact finset.mem_union_left _ h },
-    { rw not_le at hl,
-      have h₁ := drop_len_lt' (Pos g.fresh.1) hk hl,
-      have h₂ := disjoint_fresh_of_disjoint' hk hdis,
-      have h₃ : v ∈ clause.vars (drop (k - 1) l ++ [Pos g.fresh.1]),
-      { rw [clause.vars_append],
-        exact finset.mem_union_left _ h },
-      have := ih _ h₁ h₂ h₃,
-      exact finset.mem_union_right _ this } }
-end
-
-theorem not_mem_pooled_xor_vars_of_not_mem_vars_of_not_mem_stock
-  (hk : k ≥ 3) (hdis : disjoint g.stock (clause.vars l)) :
-  v ∉ (clause.vars l) → v ∉ g.stock → v ∉ (pooled_xor hk l g hdis).vars :=
-begin
-  induction l using strong_induction_on_lists with l ih generalizing g,
-  by_cases hl : length l ≤ k,
-  { rw [pooled_base_case hk hdis hl, vars_direct_xor l], tautology },
-  { intros hvars hg,
-    rw pooled_xor,
-    simp [hl],
-    rw cnf.vars_append,
-    apply finset.not_mem_union.mpr,
-    split,
-    { rw [vars_direct_xor, clause.vars_append],
-      apply finset.not_mem_union.mpr,
-      split,
-      { intro hcon,
-        have := (vars_subset_of_subset (take_subset (k - 1) l)),
-        exact absurd (this hcon) hvars },
-      { simp [var],
-        intro hcon,
-        rw hcon at hg,
-        exact absurd (fresh_mem_stock g) hg } },
-    { have h₁ := drop_len_lt' (Pos g.fresh.1) hk (not_le.mp hl),
-      have h₂ := disjoint_fresh_of_disjoint' hk hdis,
-      have h₃ : v ∉ clause.vars (drop (k - 1) l ++ [Pos g.fresh.1]),
-      { simp [clause.vars, var, clause.vars_append],
-        rintros (h | rfl),
-        { exact hvars (vars_subset_of_subset (drop_subset (k - 1) l) h) },
-        { exact hg (fresh_mem_stock g) } },
-      have h₄ : v ∉ g.fresh.2.stock,
-      { intro hcon,
-        exact hg ((fresh_stock_subset g) hcon) },
-      exact ih _ h₁ h₂ h₃ h₄ } }
-end
-
-lemma pooled_forward (hk : k ≥ 3) (hdis : disjoint g.stock (clause.vars l)) :
-  cnf.eval τ (pooled_xor hk l g hdis) = tt → cnf.eval τ (direct_xor l) = tt :=
-begin
-  induction l using strong_induction_on_lists with l ih generalizing g,
-  by_cases hl : length l ≤ k,
-  { rw pooled_base_case hk hdis hl, exact id },
-  { intro h,
-    rw pooled_xor at h,
-    simp [hl, cnf.eval_append] at h,
-    rcases h with ⟨hdir, hrec⟩,
-    have h₁ := drop_len_lt' (Pos g.fresh.1) hk (not_le.mp hl),
-    have h₂ := disjoint_fresh_of_disjoint' hk hdis,
-    have ihred := ih _ h₁ h₂ hrec,
-    rw [eval_direct_xor_eq_eval_Xor, eval_eq_bodd_count_tt] at ihred hdir |-,
-    have := congr_arg ((clause.count_tt τ)) (take_append_drop (k - 1) l).symm,
-    have := congr_arg bodd this,
-    cases hnew : (τ g.fresh.1),
-    { simp [count_tt_cons, count_tt_append, hnew, literal.eval] at ihred hdir,
-      rw [count_tt_append, bodd_add, hdir, ihred, ff_bxor] at this,
-      exact this },
-    { simp [count_tt_cons, count_tt_append, hnew, literal.eval] at ihred hdir,
-      rw [count_tt_append, bodd_add, hdir, ihred, bxor_ff] at this,
-      exact this } }
-end
-
-theorem pooled_sequiv (hk : k ≥ 3) (hdis : disjoint g.stock (clause.vars l)) :
-  sequiv (pooled_xor hk l g hdis) (direct_xor l) (clause.vars l) :=
-begin
-  induction l using strong_induction_on_lists with l ih generalizing g,
-  by_cases hl : length l ≤ k,
-  { rw pooled_base_case hk hdis hl },
-  { intro τ, split,
-    -- forward direction: pooled -> direct
-    { rintros ⟨σ, hl, hs⟩,
-      use [σ, pooled_forward hk hdis hl, hs] },
-    -- reverse direction: direct -> pooled 
-    { rintros ⟨σ, he, hs⟩,
-
-      rw [eval_direct_xor_eq_eval_Xor, eval_eq_bodd_count_tt,
-        ← (take_append_drop (k - 1) l), count_tt_append, bodd_add] at he,
-
-      have hnotmem := set.disjoint_left.mp hdis (g.fresh_mem_stock),
-      have h₁ := drop_len_lt' (Pos g.fresh.1) hk (not_le.mp hl),
-      have h₂ := disjoint_fresh_of_disjoint' hk hdis,
-
-      have htakevars := vars_subset_of_subset (take_subset (k - 1) l),
-      have hdropvars := vars_subset_of_subset (drop_subset (k - 1) l),
-
-      rw pooled_xor,
-      simp [hl, cnf.eval_append],
-
-      -- Case on the truth value of the last n - k + 1 variables
-      -- Note: the proof is symmetric, so any tightening-up can be done in both
-      cases hc : bodd (clause.count_tt σ (take (k - 1) l)),
-      { rw [hc, bool.bxor_ff_left] at he,
-        rcases exists_eqod_and_eq_of_not_mem σ ff hnotmem with ⟨γ, heqod, hg⟩,
-        have : bodd (clause.count_tt γ (drop (k - 1) l ++ [Pos g.fresh.1])) = tt,
-        { simp [count_tt_append, literal.eval, hg, cond,
-            ← count_tt_eq_of_eqod (eqod_subset hdropvars heqod), he] },
-        rw [← eval_eq_bodd_count_tt, ← eval_direct_xor_eq_eval_Xor] at this,
-
-        -- Apply the induction hypothesis
-        rcases (ih _ h₁ h₂ γ).mpr ⟨γ, this, eqod.refl _ _⟩ with ⟨γ₂, he₂, hg₂⟩,
-
-        have heqod₂ : eqod (assignment.ite (cnf.vars (pooled_xor hk (l.drop (k - 1) ++ [Pos g.fresh.1]) g.fresh.2 h₂)) γ₂ γ) γ (clause.vars l),
-        { intros v hv,
-          by_cases hmem : v ∈ clause.vars (l.drop (k - 1)),
-          { have h₃ : v ∈ clause.vars (drop (k - 1) l ++ [Pos g.fresh.1]),
-            { rw [clause.vars_append],
-              exact finset.mem_union_left _ hmem },
-            rw [ite_pos (mem_pooled_xor_vars_of_mem_vars hk h₂ h₃), hg₂ v h₃] },
-          { have hdis₂ := set.disjoint_right.mp hdis hv,
-            have hne : v ≠ g.fresh.1,
-            { intro hcon,
-              exact (hcon ▸ hdis₂) (fresh_mem_stock g) },
-            have : v ∉ clause.vars (drop (k - 1) l ++ [Pos g.fresh.1]),
-            { simp [clause.vars, var, clause.vars_append],
-              rintros (hcon | hcon),
-              { exact hmem hcon },
-              { exact hne hcon } },
-            have hstock : v ∉ g.fresh.2.stock,
-            { intro hcon,
-              exact hdis₂ ((fresh_stock_subset g) hcon) },
-            rw ite_neg (not_mem_pooled_xor_vars_of_not_mem_vars_of_not_mem_stock hk h₂ this hstock) } },
-        
-        use assignment.ite (cnf.vars (pooled_xor hk (drop (k - 1) l ++ [Pos g.fresh.1]) g.fresh.2 h₂)) γ₂ γ,
-        split,
-        { split,
-          { simp [eval_direct_xor_eq_eval_Xor, eval_eq_bodd_count_tt, 
-              count_tt_append, bodd_add, literal.eval, hg],
-            have : g.fresh.1 ∈ clause.vars (drop (k - 1) l ++ [Pos g.fresh.1]),
-            { simp [clause.vars_append, var] },
-            simp [ite_pos (mem_pooled_xor_vars_of_mem_vars hk h₂ this), 
-              ← (hg₂ g.fresh.1 this), hg,
-              count_tt_eq_of_eqod (eqod_subset htakevars heqod₂),
-              ← count_tt_eq_of_eqod (eqod_subset htakevars heqod), hc] },
-          { exact he₂ ▸ eval_eq_cnf_of_eqod (ite_eqod _ _ _) } },
-        { exact eqod.trans (eqod.trans hs heqod) heqod₂.symm } },
-      { simp only [hc, bnot_eq_true_eq_eq_ff, tt_bxor] at he,
-        rcases exists_eqod_and_eq_of_not_mem σ tt hnotmem with ⟨γ, heqod, hg⟩,
-        have : bodd (clause.count_tt γ (drop (k - 1) l ++ [Pos g.fresh.1])) = tt,
-        { simp only [count_tt_append, literal.eval, hg, cond, 
-            ← count_tt_eq_of_eqod (eqod_subset hdropvars heqod), he, bodd_succ,
-            bool.bnot_false, count_tt_singleton, bodd_succ] },
-        rw [← eval_eq_bodd_count_tt, ← eval_direct_xor_eq_eval_Xor] at this,
-
-        -- Apply the induction hypothesis
-        rcases (ih _ h₁ h₂ γ).mpr ⟨γ, this, eqod.refl _ _⟩ with ⟨γ₂, he₂, hg₂⟩,
-
-        have heqod₂ : eqod (assignment.ite (cnf.vars (pooled_xor hk (drop (k - 1) l ++ [Pos g.fresh.1]) g.fresh.2 h₂)) γ₂ γ) γ (clause.vars l),
-        { intros v hv,
-          by_cases hmem : v ∈ clause.vars (l.drop (k - 1)),
-          { have h₃ : v ∈ clause.vars (drop (k - 1) l ++ [Pos g.fresh.1]),
-            { rw [clause.vars_append],
-              exact finset.mem_union_left _ hmem },
-            rw [ite_pos (mem_pooled_xor_vars_of_mem_vars hk h₂ h₃), hg₂ v h₃] },
-          { have hdis₂ := set.disjoint_right.mp hdis hv,
-            have hne : v ≠ g.fresh.1,
-            { intro hcon,
-              exact (hcon ▸ hdis₂) (fresh_mem_stock g) },
-            have : v ∉ clause.vars (drop (k - 1) l ++ [Pos g.fresh.1]),
-            { simp [clause.vars, var, clause.vars_append],
-              rintros (hcon | hcon),
-              { exact hmem hcon },
-              { exact hne hcon } },
-            have hstock : v ∉ g.fresh.2.stock,
-            { intro hcon,
-              exact hdis₂ ((fresh_stock_subset g) hcon) },
-            rw ite_neg (not_mem_pooled_xor_vars_of_not_mem_vars_of_not_mem_stock hk h₂ this hstock) } },
-        
-        use assignment.ite (cnf.vars (pooled_xor hk (drop (k - 1) l ++ [Pos g.fresh.1]) g.fresh.2 h₂)) γ₂ γ,
-        split,
-        { split,
-          { simp [eval_direct_xor_eq_eval_Xor, eval_eq_bodd_count_tt, 
-              count_tt_append, bodd_add, literal.eval, hg],
-            have : g.fresh.1 ∈ clause.vars (drop (k - 1) l ++ [Pos g.fresh.1]),
-            { simp [clause.vars_append, var] },
-            simp [ite_pos (mem_pooled_xor_vars_of_mem_vars hk h₂ this), 
-              ← (hg₂ g.fresh.1 this), hg,
-              count_tt_eq_of_eqod (eqod_subset htakevars heqod₂),
-              ← count_tt_eq_of_eqod (eqod_subset htakevars heqod), hc] },
-          { exact he₂ ▸ eval_eq_cnf_of_eqod (ite_eqod _ _ _) } },
-        { exact eqod.trans (eqod.trans hs heqod) heqod₂.symm } } } }
-end
-
-theorem pooled_xor_encodes_Xor (hk : k ≥ 3) (hdis : disjoint g.stock (clause.vars l)) :
-  encodes Xor (pooled_xor hk l g hdis) l :=
-encodes_of_encodes_of_sequiv (direct_xor_encodes_Xor l) (pooled_sequiv hk hdis).symm
+theorem pooled_xor_encodes_Xor (hdis : disjoint g.stock (clause.vars l)) :
+  encodes Xor (pooled_xor hk l g) l :=
+tseitin_xor_encodes_Xor hk pooled_perm_is_perm hdis
 
 end tseitin_xor
